\documentclass{article}
\begin{document}
\begin{equation}
\label{ decom 1}
e^{-i \vec{q} . \vec{r}}=
4 \pi \sum_{l=0}^{\infty} 
\sum_{m=-l}^{l} i^{l} j_{l}(q r)
Y_{lm}^{*}(\theta_{r},\phi_{r}) 
Y_{lm}(\theta_{q},\phi_{q})
\end{equation}

\begin{eqnarray*}
A(\vec{q})&=&\int d^{3}x  V(\vec{r}) e^{-i \vec{q} . \vec{r}} \\
A_{lm}(q) 
\sum_{l=0}^{\infty} 
\sum_{m=-l}^{l} Y_{lm}(\theta_{q},\phi_{q}) 
 &=&\int d^{3}r  V(\vec{r}) 
4 \pi \sum_{l=0}^{\infty} 
\sum_{m=-l}^{l} i^{l} j_{l}(q r)
Y_{lm}^{*}(\theta_{r},\phi_{r}) 
Y_{lm}(\theta_{q},\phi_{q})
\\
A_{lm}(q) 
\sum_{l=0}^{\infty} 
\sum_{m=-l}^{l} Y_{lm}(\theta_{q},\phi_{q}) 
 &=&\int  dr r^{2} d\Omega  V(\vec{r}) 
4 \pi \sum_{l=0}^{\infty} 
\sum_{m=-l}^{l} i^{l} j_{l}(q r)
Y_{lm}^{*}(\theta_{r},\phi_{r}) 
Y_{lm}(\theta_{q},\phi_{q})
\\
A_{lm}(q) 
\sum_{l=0}^{\infty} 
\sum_{m=-l}^{l} Y_{lm}(\theta_{q},\phi_{q}) 
 &=&\int dr r^{2} 
4 \pi \sum_{l=0}^{\infty} 
\sum_{m=-l}^{l} i^{l} j_{l}(q r)
V_{lm}(r)
Y_{lm}(\theta_{q},\phi_{q})
\\
\end{eqnarray*}
\begin{equation}
A_{lm}=\int dr r^{2}  4 \pi i^{l} V_{lm}(r) j_{l}(q r)
\label{int 1}
\end{equation}
\end{document}
